SP1Chips/UType/Constraints.lean
@@ -7,57 +7,57 @@ namespace UType
 section constraints
 
 -- Generated Lean code for chip UTypeChip
-@[irreducible] def constraints (Main : Vector (Fin KB) 31) : SP1ConstraintList (Fin KB) :=
-  let E0 : Fin KB := Main[30] - 1
-  let E1 : Fin KB := Main[30] * E0
-  let E2 : Fin KB := Main[29] - 1
-  let E3 : Fin KB := Main[29] * E2
-  let E4 : Fin KB := Main[29] * 48
-  let E5 : Fin KB := 1 - Main[29]
-  let E6 : Fin KB := E5 * 49
-  let E7 : Fin KB := E4 + E6
-  let E8 : Fin KB := 1 - Main[29]
-  let E9 : Fin KB := Main[29] * 0
-  let E10 : Fin KB := E8 * 0
-  let E11 : Fin KB := E9 + E10
-  let E12 : Fin KB := Main[29] * 0
-  let E13 : Fin KB := E8 * 0
-  let E14 : Fin KB := E12 + E13
-  let E15 : Fin KB := Main[29] * 23
-  let E16 : Fin KB := E8 * 55
-  let E17 : Fin KB := E15 + E16
-  let E18 : Fin KB := Main[29] * 128
-  let E19 : Fin KB := E8 * 128
-  let E20 : Fin KB := E18 + E19
-  let E21 : Fin KB := Main[3] + 4
-  let CS0 : SP1ConstraintList (Fin KB) := CPUState.constraints { clk_high := Main[0], clk_16_24 := Main[1], clk_0_16 := Main[2], pc := #v[Main[3], Main[4], Main[5]] } #v[E21, Main[4], Main[5]] 8 Main[30]
-  let E22 : Fin KB := Main[29] * Main[3]
-  let E23 : Fin KB := 1 - Main[29]
-  let E24 : Fin KB := E23 * 0
-  let E25 : Fin KB := E22 + E24
-  let E26 : Fin KB := Main[29] * Main[4]
-  let E27 : Fin KB := 1 - Main[29]
-  let E28 : Fin KB := E27 * 0
-  let E29 : Fin KB := E26 + E28
-  let E30 : Fin KB := Main[29] * Main[5]
-  let E31 : Fin KB := 1 - Main[29]
-  let E32 : Fin KB := E31 * 0
-  let E33 : Fin KB := E30 + E32
-  let E34 : Fin KB := Main[29] * 0
-  let E35 : Fin KB := 1 - Main[29]
-  let E36 : Fin KB := E35 * 0
-  let E37 : Fin KB := E34 + E36
-  let E38 : Fin KB := Main[22] - E25
-  let E39 : Fin KB := Main[23] - E29
-  let E40 : Fin KB := Main[24] - E33
-  let E41 : Fin KB := 0 - E37
-  let E42 : Fin KB := Main[30] - 1
-  let E43 : Fin KB := E42 * Main[13]
-  let E44 : Fin KB := Main[30] - Main[13]
-  let CS1 : SP1ConstraintList (Fin KB) := AddOperation.constraints #v[Main[22], Main[23], Main[24], 0] #v[Main[14], Main[15], Main[16], Main[17]] { value := #v[Main[25], Main[26], Main[27], Main[28]] } E44
-  let E45 : Fin KB := Main[1] * 65536
-  let E46 : Fin KB := Main[2] + E45
-  let CS2 : SP1ConstraintList (Fin KB) := JTypeReader.constraints Main[0] E46 #v[Main[3], Main[4], Main[5]] E7 #v[E20, E17, E11, E14] #v[Main[25], Main[26], Main[27], Main[28]] { op_a := Main[6], op_a_memory := { prev_value := #v[Main[7], Main[8], Main[9], Main[10]], access_timestamp := { prev_low := Main[11], diff_low_limb := Main[12] } }, op_a_0 := Main[13], op_b_imm := #v[Main[14], Main[15], Main[16], Main[17]], op_c_imm := #v[Main[18], Main[19], Main[20], Main[21]] } Main[30]
+@[irreducible] def constraints {F : Type} [Field F] [CoeHead F ℕ] (Main : Vector F 31) : SP1ConstraintList F :=
+  let E0 : F := Main[30] - 1
+  let E1 : F := Main[30] * E0
+  let E2 : F := Main[29] - 1
+  let E3 : F := Main[29] * E2
+  let E4 : F := Main[29] * 48
+  let E5 : F := 1 - Main[29]
+  let E6 : F := E5 * 49
+  let E7 : F := E4 + E6
+  let E8 : F := 1 - Main[29]
+  let E9 : F := Main[29] * 0
+  let E10 : F := E8 * 0
+  let E11 : F := E9 + E10
+  let E12 : F := Main[29] * 0
+  let E13 : F := E8 * 0
+  let E14 : F := E12 + E13
+  let E15 : F := Main[29] * 23
+  let E16 : F := E8 * 55
+  let E17 : F := E15 + E16
+  let E18 : F := Main[29] * 128
+  let E19 : F := E8 * 128
+  let E20 : F := E18 + E19
+  let E21 : F := Main[3] + 4
+  let CS0 : SP1ConstraintList F := CPUState.constraints { clk_high := Main[0], clk_16_24 := Main[1], clk_0_16 := Main[2], pc := #v[Main[3], Main[4], Main[5]] } #v[E21, Main[4], Main[5]] 8 Main[30]
+  let E22 : F := Main[29] * Main[3]
+  let E23 : F := 1 - Main[29]
+  let E24 : F := E23 * 0
+  let E25 : F := E22 + E24
+  let E26 : F := Main[29] * Main[4]
+  let E27 : F := 1 - Main[29]
+  let E28 : F := E27 * 0
+  let E29 : F := E26 + E28
+  let E30 : F := Main[29] * Main[5]
+  let E31 : F := 1 - Main[29]
+  let E32 : F := E31 * 0
+  let E33 : F := E30 + E32
+  let E34 : F := Main[29] * 0
+  let E35 : F := 1 - Main[29]
+  let E36 : F := E35 * 0
+  let E37 : F := E34 + E36
+  let E38 : F := Main[22] - E25
+  let E39 : F := Main[23] - E29
+  let E40 : F := Main[24] - E33
+  let E41 : F := 0 - E37
+  let E42 : F := Main[30] - 1
+  let E43 : F := E42 * Main[13]
+  let E44 : F := Main[30] - Main[13]
+  let CS1 : SP1ConstraintList F := AddOperation.constraints #v[Main[22], Main[23], Main[24], 0] #v[Main[14], Main[15], Main[16], Main[17]] { value := #v[Main[25], Main[26], Main[27], Main[28]] } E44
+  let E45 : F := Main[1] * 65536
+  let E46 : F := Main[2] + E45
+  let CS2 : SP1ConstraintList F := JTypeReader.constraints Main[0] E46 #v[Main[3], Main[4], Main[5]] E7 #v[E20, E17, E11, E14] #v[Main[25], Main[26], Main[27], Main[28]] { op_a := Main[6], op_a_memory := { prev_value := #v[Main[7], Main[8], Main[9], Main[10]], access_timestamp := { prev_low := Main[11], diff_low_limb := Main[12] } }, op_a_0 := Main[13], op_b_imm := #v[Main[14], Main[15], Main[16], Main[17]], op_c_imm := #v[Main[18], Main[19], Main[20], Main[21]] } Main[30]
   CS0 ++ CS1 ++ CS2 ++ [
     (.assertZero E1),
     (.assertZero E3),
